playground/uart_model/tests/simplify_decomp.sml
@@ -1,0 +1,220 @@
+(*
+    loadPath := ("/home/daniil/Apps/HOL/examples/l3-machine-code/m0/decompiler"::(!loadPath));
+    loadPath := ("/home/daniil/Apps/HOL/examples/l3-machine-code/m0/prog"::(!loadPath));
+    loadPath := ("/Home/daniil/Apps/HOL/examples/l3-machine-code/common"::(!loadPath));
+    loadPath := ("/home/daniil/projects/Kvasir/playground/uart_model/helpers"::(!loadPath));
+    loadPath := ("/home/daniil/projects/Kvasir/playground/uart_model/nit2bisim"::(!loadPath));
+    loadPath := ("/home/daniil/projects/Kvasir/playground/uart_model/prog"::(!loadPath));
+*)
+open m0_progTheory
+open wordsLib
+open m0_decompLib
+
+
+
+fun simplifySpec sp=  sp |>(I ## (fn x =>  x|> SIMP_RULE (arith_ss++ boolSimps.CONJ_ss++boolSimps.LET_ss ++WORD_ss++WORD_EXTRACT_ss)
+                 [
+                    GSYM CONJ_ASSOC,
+                  combinTheory.UPDATE_APPLY
+                  ]))
+                        
+                        
+val spec =  
+`(*movs r1, #0
+movs r2, #100*)
+movs r3, #4
+label:
+ldrb r4, [r1, r3]
+ldrb r5, [r2, r3]
+eors r4, r5
+strb r4, [r6, r3]
+subs r3, r3, #1
+bne label
+`
+ |> (m0_decompile_code "simpleOTP")
+ |> simplifySpec
+;
+
+
+val spec =`
+movs r1, #100
+ldrb r2, [r3, #0]
+strb r2, [r6, #0]
+ldrb r2, [r3, #1]
+strb r2, [r6, #1]
+ldrb r2, [r3, #2]
+strb r2, [r6, #2]
+`|> (m0_decompile_code "simpleOTP")
+ |> simplifySpec
+;
+
+val spec =`
+movs r2, #100
+strb r2, [r1, #0]
+strb r2, [r1, #1]
+strb r2, [r1, #2]
+strb r2, [r1, #3]
+strb r2, [r1, #4]
+strb r2, [r1, #5]
+`|> (m0_decompile_code "simpleOTP")
+ |> simplifySpec
+;
+
+val spec = `
+movs r1, #0
+movs r2, #100 
+ldrb r3, [r1, #0]
+ldrb r4, [r2, #0]
+eors r3, r4
+strb r3, [r1, #0]
+
+ldrb r3, [r1, #1]
+ldrb r4, [r2, #1]
+eors r3, r4
+strb r3, [r1, #1]
+
+ldrb r3, [r1, #2]
+ldrb r4, [r2, #2]
+eors r3, r4
+strb r3, [r1, #2]
+
+ldrb r3, [r1, #3]
+ldrb r4, [r2, #3]
+eors r3, r4
+strb r3, [r1, #3]
+
+ldrb r3, [r1, #4]
+ldrb r4, [r2, #4]
+eors r3, r4
+strb r3, [r1, #4]
+
+ldrb r3, [r1, #5]
+ldrb r4, [r2, #5]
+eors r3, r4
+strb r3, [r1, #5]
+
+
+ldrb r3, [r1, #6]
+ldrb r4, [r2, #6]
+eors r3, r4
+strb r3, [r1, #6]
+
+ldrb r3, [r1, #7]
+ldrb r4, [r2, #7]
+eors r3, r4
+strb r3, [r1, #7]
+
+
+ldrb r3, [r1, #8]
+ldrb r4, [r2, #8]
+eors r3, r4
+strb r3, [r1, #8]
+
+ldrb r3, [r1, #9]
+ldrb r4, [r2, #9]
+eors r3, r4
+strb r3, [r1, #9]
+`|> (m0_decompile_code "simpleOTP")
+ |> simplifySpec
+;
+DB.find "m0_MEMORY"
+
+
+
+
+
+val test_thm =prove(``!x y dmem.(x<>y)/\(x IN dmem ==> x IN (dmem DELETE y))``, cheat)
+
+val mem_trm = mk_var("mem", mk_int_word_type 32 --> mk_int_word_type 8)
+val mem_split = prove( (*subst [``mem':word32->word8``|->mem_trm]*) ``!c.c IN dm ==> (m0_MEMORY dm (m:word32-> word8) = m0_MEM (c) (m c) * m0_MEMORY (dmem DELETE c) m)``, cheat) 
+
+val c = a |> REWRITE_RULE [b]
+  |> SIMP_RULE (std_ss++boolSimps.LET_ss ++boolSimps.CONJ_ss) [SPEC_MOVE_COND]
+  |> SIMP_RULE (bool_ss++pred_setLib.PRED_SET_ss) [test_thm, m0_MEMORY_INSERT |> GSYM |> GEN_ALL];
+
+set_trace "simplifier" 2
+
+  c |> SIMP_RULE (bool_ss++pred_setLib.PRED_SET_ss) [test_thm, m0_MEMORY_INSERT |> GSYM |> GEN_ALL];
+  c |> SIMP_RULE (bool_ss) [mem_split]
+    |> SIMP_RULE (arith_ss++boolSimps.LET_ss ++WORD_ss++WORD_EXTRACT_ss)
+                 [
+                    GSYM CONJ_ASSOC,
+                  combinTheory.UPDATE_APPLY
+                  ]
+  |> SIMP_RULE (std_ss) [GSYM set_sepTheory.SEP_ARRAY_def, ]
+
+
+  
+
+
+(* would be nice to firther simplify things by expresing this as a function on SEP_ARRAYS *)
+set_sepTheory.SEP_ARRAY_def
+
+
+
+
+val test_thm= prove(``
+ !a b c x y f. a <> b ==> ( (b=+y)((a=+x)f) =((c =+ y) o (a =+ x)) f  )
+``,cheat)
+
+
+
+
+spec |>(I ## (fn x =>  x|> SIMP_RULE (arith_ss++boolSimps.LET_ss ++WORD_ss++WORD_EXTRACT_ss)
+                 [
+ (*                 BBLAST_CONV ``!r1.r1:word32 <> r1+1w``,
+                  BBLAST_CONV ``!r1.(r1:word32)+1w <> r1+2w``,*)
+                  combinTheory.UPDATE_APPLY]))
+
+
+`` ((1w =+ mem 1w ?? mem 101w)       ((0w =+ mem 0w ?? mem 100w) mem)``
+
+
+``(x:word32) ?? (x:word32)``
+
+
+
+          
+
+
+open blastLib
+  bool_simsLib.LET_ss
+val (m0_encrypt_th, m0_encrypt_defs) = m0_decompile "m0_encrypt"`
+ 00c0   (* lsls	r0, r0, #3	*)
+ 5c14   (* ldrb	r4, [r2, r0]	*)
+ 788b   (* ldrb	r3, [r1, #2]	*)
+ 1812   (* adds	r2, r2, r0	*)
+ 4063   (* eors	r3, r4		*)
+ 708b   (* strb	r3, [r1, #2]	*)
+ 7850   (* ldrb	r0, [r2, #1]	*)
+ 78cb   (* ldrb	r3, [r1, #3]	*)
+ 4043   (* eors	r3, r0		*)
+ 70cb   (* strb	r3, [r1, #3]	*)
+ 7890   (* ldrb	r0, [r2, #2]	*)
+ 790b   (* ldrb	r3, [r1, #4]	*)
+ 4043   (* eors	r3, r0		*)
+ 710b   (* strb	r3, [r1, #4]	*)
+ 78d0   (* ldrb	r0, [r2, #3]	*)
+ 794b   (* ldrb	r3, [r1, #5]	*)
+ 4043   (* eors	r3, r0		*)
+ 714b   (* strb	r3, [r1, #5]	*)
+ 7910   (* ldrb	r0, [r2, #4]	*)
+ 798b   (* ldrb	r3, [r1, #6]	*)
+ 4043   (* eors	r3, r0		*)
+ 718b   (* strb	r3, [r1, #6]	*)
+ 7950   (* ldrb	r0, [r2, #5]	*)
+ 79cb   (* ldrb	r3, [r1, #7]	*)
+ 4043   (* eors	r3, r0		*)
+ 71cb   (* strb	r3, [r1, #7]	*)
+ 7990   (* ldrb	r0, [r2, #6]	*)
+ 7a0b   (* ldrb	r3, [r1, #8]	*)
+ 4043   (* eors	r3, r0		*)
+ 720b   (* strb	r3, [r1, #8]	*)
+ 79d2   (* ldrb	r2, [r2, #7]	*)
+ 7a4b   (* ldrb	r3, [r1, #9]	*)
+ 4053   (* eors	r3, r2		*)
+ 724b   (* strb	r3, [r1, #9]	*)
+`;
+
+
+ 
