playground/uart_model/clock/clockScript.sml
@@ -13,7 +13,10 @@ val simpAll =  ((DB.find "dfn'") |> map (fst o snd ) |> fs  )>>
     fs[m0Theory.CallSupervisor_def, m0Theory.Raise_def, Raise'_def]
 (* clock count in rel_sequance ether increeses monotonically, or execution stals  *)
     
-val NEX_MONO  = Q.store_thm("NEX_MONO",`!s. (s.count < (Next s).count) 
+val  NEXT_MONO = Q.store_thm("NEXT_MONO",
+`!s. s.count <= (Next s).count`,
+    cheat);
+val NEX_SMONO  = Q.store_thm("NEX_MONO",`!s. (s.count < (Next s).count) 
                     \/ ( (Next s).exception <> NoException)`,
     strip_tac>>
     Q.ABBREV_TAC `s'= Next s`>>
@@ -39,7 +42,7 @@ val NEX_MONO  = Q.store_thm("NEX_MONO",`!s. (s.count < (Next s).count)
 );
 
 
-val SEQ_MONO_AXI = Q.store_thm("SEQ_MONO_AXI", 
+val SEQ_SMONO_AXI = Q.store_thm("SEQ_MONO_AXI", 
         `!s i seq. 
             rel_sequence (NEXT_REL $= NextStateM0) seq s 
                 ==> (((seq i).count < (seq (i+1)).count) 
@@ -53,62 +56,18 @@ val SEQ_MONO_AXI = Q.store_thm("SEQ_MONO_AXI",
     ` by METIS_TAC[])>>
 
     Tactical.REVERSE(Cases_on `(Next (seq i)).exception = NoException`>> fs[])>-(
-            fs[DECIDE``i+1=SUC i``, NEX_MONO]
+            fs[DECIDE``i+1=SUC i``, NEX_SMONO]
     )>>
     DISJ1_TAC>>
-    fs[DECIDE``i+1=SUC i``, NEX_MONO]>>
-    METIS_TAC[NEX_MONO]
+    fs[DECIDE``i+1=SUC i``, NEX_SMONO]>>
+    METIS_TAC[NEX_SMONO]
 );
 
-    
-                   
-
-(* next is strictly monotonically increasing in clock cycles *)
-(*		  
-    REPEAT STRIP_TAC 
-    Q.ABBREV_TAC `sf = Next s`
-    FULL_SIMP_TAC (std_ss++LET_ss) [Next_def]
-    Q.ABBREV_TAC `s1 = Fetch s`>>
-    Cases_on `s1`>>
-    FULL_SIMP_TAC (std_ss++LET_ss) [Next_def]>>
-    Q.ABBREV_TAC `s2 = Decode q r`
-    Cases_on `s2`
-`(!x. inst<> Undefined x) ==> s.count < (Run inst s).count` by cheat
-`!x. (inst= Undefined x) ==>  ((Run inst s).pending=(SOME HardFault))` by cheat
-
-    FULL_SIMP_TAC (std_ss++LET_ss) [Run_def]>>
-
-    Cases_on `q'`>>
-    (
-FULL_SIMP_TAC (std_ss++LET_ss) [instruction_case_def, BranchTo_def,						IncPC_def, write'PC_def,
-dfn'Undefined_def,
-Raise_def,
-dfn'NoOperation_def]
-    )
+val SEQ_EXISTS_PREV_STATE_thm = Q.store_thm("SEQ_EXISTS_PREV_STATE_thm", 
+        `!s i seq. 
+            rel_sequence (NEXT_REL $= NextStateM0) seq s /\ (seq i).count > (seq 0).count==> ? i'. (seq i').count < (seq i).count /\ ((seq (i'+1)) = (seq i)) `,
+        cheat
 );
-*)
-(*
-val  NEXT_MONO = Q.store_thm("NEXT_MONO",
-`!s. s.count <= (Next s).count`,
-    cheat);
-SIMP_TAC std_ss [Next_def]
-DB.find "DecodeThumb_def"
-DB.find "dnf'NO"
-EVAL ``ARB+1n``
-
-DB.find "Run_def"
-DB.find "unpredictable"
-DB.find "dfn'BranchExchange"
-(* also works thus far:  
-`!s. s.count <= (Next s).count`,
-*)
-);
-				
-DB.find "Exception"
-ExceptionEntry
-ExceptionTaken
-ExceptionReturn
-
 (*
 execution sequences are strictly monotonically increasing
 in clock cycles
@@ -151,7 +110,7 @@ val SEQ_MONO_B = Q.store_thm("SEQ_MONO_B",
     MP_TAC (Q.SPECL [`s`, `a`, `b-a`, `seq`] SEQ_MONO2)>>
     FULL_SIMP_TAC arith_ss []
 );
-
+(*
 val SEQ_UNIQUE1 = Q.prove(
 `!s i seq. rel_sequence (NEXT_REL $= NextStateM0) seq s /\ ( (seq i).count = (seq (i+1)).count)  ==>
 (seq i = seq (i+1))
