playground/uart_model/nit2bisim/nit2bisim2Script.sml
@@ -1,0 +1,261 @@
+(*
+         loadPath := ("../uart"::(!loadPath));
+         loadPath := ("../prog"::(!loadPath));
+         loadPath := ("../clock"::(!loadPath));
+ *)
+open HolKernel Parse boolLib bossLib;
+open m0_NITTheory
+open uartTheory
+open m0u_progTheory
+open m0_progTheory
+open stateTheory m0_stepTheory;
+open boolSimps;
+open pred_setTheory;
+open m0_progTheory;
+open pairTheory;
+open progTheory;
+open set_sepTheory;
+open clockTheory;
+
+val _ = new_theory "nit2bisim2";
+
+(********************************************)
+(*          No exceptions                   *)
+(*                                          *)
+(********************************************)
+
+(* There will be no exceptions for t clock 
+   cycles executing from a state constrained by P *)
+
+val NEX_def = Define `
+    NEX (P :(m0_component # m0_data -> bool) -> bool) t = ! s seq i.    
+               ((SEP_REFINE (P * SEP_T) ($=) (STATE m0_proj) s) /\
+               rel_sequence (NEXT_REL $= NextStateM0) seq  s /\
+               ((seq (i)).count < s.count+ t))==>   
+	           ((seq i).count < (Next(seq i)).count) /\
+                   ((Next (seq (i))).exception = NoException) `;
+
+val NEX_VERI_0_thm= Q.store_thm("NEX_VERI_0_thm",
+`!P. NEX P 0`,
+    fs[NEX_def]>>
+    REPEAT strip_tac>>
+    (`(s).count ≤ (seq i).count` by
+        METIS_TAC[SEQ_MONO_B, DECIDE ``0n<=i``, 
+                  rel_sequence_def, NEXT_REL_def,
+                  NextStateM0_def]
+        )>>
+    fs[]
+);
+
+
+
+(* This is our strong non interference property
+   After executing t clock cycles no information flow to or from the region can be observed
+   in each step
+*)
+val NIT_def = Define`
+NIT region(P :(m0_component # m0_data -> bool) -> bool)  t =   !s s' seq seq' i.   
+               ((SEP_REFINE (P * SEP_T) ($=) (STATE m0_proj) s) /\
+               m0_non_r_eq region s s' /\ 
+               rel_sequence (NEXT_REL $= NextStateM0) seq  s /\
+               rel_sequence (NEXT_REL $= NextStateM0) seq' s' /\
+               ((seq i).count < s.count+t)) ==>   
+                   m0_non_r_eq region (seq (SUC i)) (seq' (SUC i)) /\
+                   m0_r_eq region (seq' 0) (seq' (SUC i))
+`;
+
+
+
+
+val NIT_NIT_STEP_thm = store_thm("NIT_NIT_STEP_thm",
+``  ! P t region. 
+        ((NEX P t)/\ (NIT region P t)) = ! s seq i . (
+        SEP_REFINE (P * SEP_T) $= (STATE m0_proj) s /\
+        rel_sequence (NEXT_REL $= NextStateM0) seq s /\
+        (seq i).count < s.count + t ==> NIT_STEP region (seq i))``,
+        cheat
+);
+
+(* bisim *)
+val SEQ_MONO_LEM = Q.prove( `!seq s i t.
+    (rel_sequence (NEXT_REL $= NextStateM0) seq s)/\
+    ((seq (SUC i)).count < s.count + t)==> ((seq i).count < s.count + t)`,
+    REPEAT GEN_TAC>>
+    (MP_TAC o Q.SPECL[`s`,`i`,`SUC i`,`seq`] ) SEQ_MONO_B>>
+    ASM_SIMP_TAC std_ss []>>
+    METIS_TAC [ DECIDE ``( x:num <= y:num /\ y < z:num ) ==> (x < z) ``]
+);
+
+val COSIM'_def = Define `COSIM' P t = ! s s' seq seq' i.
+    ((SEP_REFINE (P * SEP_T) ($=) (STATE m0_proj) s) /\
+    rel_sequence (NEXT_REL $= NextStateM0) seq  s /\
+    rel_sequence (NEXT_REL $= NextStateM0U) seq' s' /\
+    m0u_m0_non_r_eq uart_r s' s /\ ((seq i).count < s.count + t) )==>
+        m0u_m0_non_r_eq uart_r (m0u_Next (seq' i)) (Next (seq i)) /\
+        m0u_r_eq uart_r (seq' i)  (m0u_Next (seq' i))`;
+
+val COSIM''_def = Define `COSIM'' P t = ! s s' seq seq' i.
+    ((SEP_REFINE (P * SEP_T) ($=) (STATE m0_proj) s) /\
+    rel_sequence (NEXT_REL $= NextStateM0) seq  s /\
+    rel_sequence (NEXT_REL $= NextStateM0U) seq' s' /\
+    m0u_m0_non_r_eq uart_r s' s /\ ((seq i).count < s.count + t) )==>
+        m0u_m0_non_r_eq uart_r (seq' (SUC i)) (seq (SUC i)) /\
+        m0u_r_eq uart_r (seq' i)  (seq' (SUC i))`;
+
+val COSIM_def = Define `COSIM P t = ! s s' seq seq' i.
+    ((SEP_REFINE (P * SEP_T) ($=) (STATE m0_proj) s) /\
+    rel_sequence (NEXT_REL $= NextStateM0) seq  s /\
+    rel_sequence (NEXT_REL $= NextStateM0U) seq' s' /\
+    m0u_m0_non_r_eq uart_r s' s /\ ((seq i).count <= s.count + t) )==>
+        m0u_m0_non_r_eq uart_r (seq' ( i)) (seq ( i)) /\
+        m0u_r_eq uart_r (seq' 0)  (seq' ( i))`;
+
+
+val cosim_def = Define `cosim P c t = COSIM ((CODE_POOL m0_instr c) * P  ) t`;
+
+val NEX_thm = Q.store_thm("NEX_thm",
+    `! P t s seq i. 
+        (NEX P t) ==> 
+            SEP_REFINE (P * SEP_T) $= (STATE m0_proj) s /\
+            rel_sequence (NEXT_REL $= NextStateM0) seq s /\
+            (seq (i)).count < s.count + t ==>
+                ((seq i).count < (Next(seq i)).count) /\ ((Next (seq i)) = (seq(SUC i)))`,
+    REPEAT GEN_TAC>>
+    STRIP_TAC>>
+    REPEAT GEN_TAC>>
+    Induct_on `i` >- (
+        STRIP_TAC>>
+        `(seq 0).count < (Next (seq 0)).count ∧
+        ((Next (seq 0)).exception = NoException)` by METIS_TAC[NEX_def]>>
+        FULL_SIMP_TAC std_ss [NEX_def, rel_sequence_def, NEXT_REL_def, NextStateM0_def, LET_DEF]>>
+        `Next (seq 0) = seq (SUC 0)` by METIS_TAC[]>>
+        REV_FULL_SIMP_TAC std_ss []
+    )>>
+    STRIP_TAC>>
+    `(seq (SUC i)).count < (Next (seq (SUC i))).count ∧
+    ((Next (seq (SUC i))).exception = NoException)` by METIS_TAC[NEX_def, SEQ_MONO_LEM]>>
+    FULL_SIMP_TAC std_ss [NEX_def, rel_sequence_def, NEXT_REL_def, NextStateM0_def, LET_DEF]>>
+    METIS_TAC[]
+);
+
+val PRODUCT_STATE_lem = prove(``!s z_i. ?z_0. m0_non_r_eq uart_r s z_0 /\ m0_r_eq uart_r z_0 z_i``,
+    REPEAT GEN_TAC>>
+    EXISTS_TAC ``s with <|MEM := (\x. if (x IN uart_r)
+                                         then (z_i.MEM x)
+                                         else (s.MEM x)) |>``>>
+    SIMP_TAC (std_ss++pred_setLib.PRED_SET_ss) [m0Theory.m0_state_accfupds,
+                m0_non_r_eq_def, m0_r_eq_def, mem_eq_def]
+);
+
+val eq_lem = prove(``!a b r.
+    m0_non_r_eq r a  b /\ m0_r_eq r a b ==> (a=b)``,
+
+    REPEAT GEN_TAC>>
+    Cases_on `a`>>Cases_on `b`>>
+    SIMP_TAC (std_ss++pred_setLib.PRED_SET_ss) [m0Theory.m0_state_accfupds,
+m0Theory.m0_state_accessors,m0_non_r_eq_def, m0_r_eq_def, mem_eq_def, m0Theory.m0_state_11]>>
+    Cases_on  `x NOTIN r ` >> METIS_TAC[]
+);
+
+
+val LEM = prove(
+    ``!(a:((m0_state # uart_state) # word32 list # word32 list))
+       (b:((m0_state # uart_state) # word32 list # word32 list)) region.
+            m0u_r_eq region a b ==> ((SND (FST a)) = (SND (FST b)))``,
+    Cases_on `a`>> Cases_on `b`>> Cases_on `q`>>
+    Cases_on `q'`>> Cases_on `r`>> Cases_on `r'`>>
+    SIMP_TAC std_ss [m0u_r_eq_def]
+);
+
+
+val LEM1 = prove(
+    ``!a b region. (m0u_m0_non_r_eq  region a b) ==>
+        (((FST o FST) a).count =  b.count)/\
+        (((FST o FST) a).exception =  b.exception)``,
+    Cases_on `a`>> Cases_on `q`>> Cases_on `r`>>
+    SIMP_TAC std_ss [m0u_m0_non_r_eq_def, m0_non_r_eq_def]
+);
+
+
+val NIT_COSIM'_thm = Q.store_thm ("NIT_COSIM'_thm",
+    `!P t.  ((NIT uart_r P t) /\ (NEX P t)) ==> (COSIM' P t)`,
+    SIMP_TAC std_ss [ COSIM'_def, PULL_FORALL]>>
+    REPEAT GEN_TAC>>
+    STRIP_TAC>>
+    STRIP_TAC>>
+    Induct_on `i` >-
+    (
+        STRIP_TAC>>
+        `((seq 0).count < (Next (seq 0)).count) ∧( (Next (seq 0) = seq (SUC 0)))` by
+            METIS_TAC[NEX_thm]>>
+        `NIT_STEP uart_r (seq 0)` by METIS_TAC[NIT_NIT_STEP_thm]>>
+        METIS_TAC[rel_sequence_def, AXI, m0u_r_eq_antisym_thm]
+    )>>
+    STRIP_TAC >>
+    `(seq i).count < s.count + t` by (
+        METIS_TAC[SEQ_MONO_LEM]
+    )>>
+    FULL_SIMP_TAC std_ss []>>
+    ` (seq i).count < (Next (seq i)).count ∧
+    (Next (seq i) = seq (SUC i))` by METIS_TAC[NEX_thm]>>
+    ` (seq (SUC i)).count < (Next (seq (SUC i))).count ∧
+    (Next (seq (SUC i)) = seq (SUC(SUC i)))` by METIS_TAC[NEX_thm]>>
+    `NIT_STEP uart_r (seq (SUC i) )` by METIS_TAC[NIT_NIT_STEP_thm]>>
+    `m0u_Next (seq' i) =  (seq' (SUC i))` by (
+        ` ((FST ∘ FST) (m0u_Next (seq' i))).exception = NoException` by METIS_TAC[LEM1,NEX_def]>>
+        `if ∃x. NEXT_REL $= NextStateM0U (seq' i) x then
+               NEXT_REL $= NextStateM0U (seq' i) (seq' (SUC i))
+             else seq' (SUC i) = seq' i` by METIS_TAC [rel_sequence_def]>>
+        rfs[rel_sequence_def, NextStateM0U_def,
+                               NEXT_REL_def, LET_DEF, PULL_EXISTS]
+    )>>
+    METIS_TAC [m0u_r_eq_antisym_thm, AXI]
+);
+
+
+val NIT_COSIM''_thm = Q.prove(`!P t.  ((NIT uart_r P t) /\ (NEX P t)) ==> (COSIM'' P t)`,
+    fs[COSIM''_def, PULL_FORALL]>>
+    REPEAT gen_tac>> strip_tac >>strip_tac>>
+    `COSIM' P t` by fs[NIT_COSIM'_thm]>>
+    ` m0u_m0_non_r_eq uart_r (m0u_Next (seq' i)) (Next (seq i)) ∧
+             m0u_r_eq uart_r (seq' i) (m0u_Next (seq' i))` by ( 
+        fs[COSIM'_def]>> METIS_TAC[]
+    )>>
+    (`Next (seq i) = seq (SUC i)` by(
+        (mp_tac (Q.SPECL [`P`, `t`, `s`, `seq`, `i`] NEX_thm))>>
+        fs[]))>>
+    `m0u_Next (seq' i) = seq' (SUC i)` by (
+        (`((Next (seq i)).exception = NoException)` by (
+            fs[NEX_def] >>
+            METIS_TAC[])
+        )>>
+        (`(((FST ∘ FST)(m0u_Next (seq' i))).exception = NoException)` by METIS_TAC[LEM1])>>
+        rfs[NextStateM0U_def, rel_sequence_def, NEXT_REL_def]>>
+        `m0u_Next (seq' i) = seq' (SUC i)` by METIS_TAC[]
+    )>>
+    fs[]
+);
+
+val NIT_COSIM_thm = Q.store_thm ("NIT_COSIM_thm",
+    `!P t.  ((NIT uart_r P t) /\ (NEX P t)) ==> (COSIM P t)`,
+                           (* use NIT_COSIM''_thm *)
+    cheat);
+     
+(* 
+`!P t.  ((NIT uart_r P t) /\ (NEX P t)) ==> (COSIM2 P t)`,
+        REPEAT STRIP_TAC >>
+       `COSIM P t ` by fs[ NIT_COSIM_thm]>> 
+       fs[COSIM2_def] >> 
+        REPEAT GEN_TAC >>
+             
+       STRIP_TAC
+       Q.PAT_X_ASSUM `COSIM P t` ( MP_TAC o Q.SPECL [`s`, `s'`, `seq`, `seq'`, `i`] o REWRITE_RULE [COSIM_def] )
+
+
+
+       (MP_TAC o Q.SPECL [`P`, `t`])  NEX_thm
+       fs[NEX_thm]
+       STRIP_TAC
+       METIS_TAC[]
+*)
+val _ = export_theory();
